cedar-lean/Cedar/Spec/Entities.lean
@@ -14,7 +14,9 @@
  limitations under the License.
 -/
 
-import Cedar.Spec.Value
+module
+
+public import Cedar.Spec.Value
 
 /-!
 This file defines Cedar entities.
@@ -26,38 +28,38 @@ open Cedar.Data
 
 ----- Definitions -----
 
-abbrev Tag := String
+public abbrev Tag := String
 
-structure EntityData where
+public structure EntityData where
   attrs : Map Attr Value
   ancestors : Set EntityUID
   tags : Map Tag Value
 
-abbrev Entities := Map EntityUID EntityData
+public abbrev Entities := Map EntityUID EntityData
 
-def Entities.ancestors (es : Entities) (uid : EntityUID) : Result (Set EntityUID) := do
+public def Entities.ancestors (es : Entities) (uid : EntityUID) : Result (Set EntityUID) := do
   let d ← es.findOrErr uid .entityDoesNotExist
   .ok d.ancestors
 
-def Entities.ancestorsOrEmpty (es : Entities) (uid : EntityUID) : Set EntityUID :=
+public def Entities.ancestorsOrEmpty (es : Entities) (uid : EntityUID) : Set EntityUID :=
   match es.find? uid with
   | some d => d.ancestors
   | none   => Set.empty
 
-def Entities.attrs (es : Entities) (uid : EntityUID) : Result (Map Attr Value) := do
+public def Entities.attrs (es : Entities) (uid : EntityUID) : Result (Map Attr Value) := do
   let d ← es.findOrErr uid .entityDoesNotExist
   .ok d.attrs
 
-def Entities.attrsOrEmpty (es : Entities) (uid : EntityUID) : Map Attr Value :=
+public def Entities.attrsOrEmpty (es : Entities) (uid : EntityUID) : Map Attr Value :=
   match es.find? uid with
   | some d => d.attrs
   | none   => Map.empty
 
-def Entities.tags (es : Entities) (uid : EntityUID) : Result (Map Tag Value) := do
+public def Entities.tags (es : Entities) (uid : EntityUID) : Result (Map Tag Value) := do
   let d ← es.findOrErr uid .entityDoesNotExist
   .ok d.tags
 
-def Entities.tagsOrEmpty (es : Entities) (uid : EntityUID) : Map Tag Value :=
+public def Entities.tagsOrEmpty (es : Entities) (uid : EntityUID) : Map Tag Value :=
   match es.find? uid with
   | some d => d.tags
   | none   => Map.empty
