cedar-lean/Cedar/Spec/Ext/Util.lean
@@ -1,3 +1,5 @@
+module
+
 namespace Cedar.Spec.Ext
 
 ----- Helper Functions -----
@@ -6,12 +8,12 @@ namespace Cedar.Spec.Ext
 Helper function that wraps String.toInt? but returns .none if the string contains '_'.
 This prevents the undocumented behavior where String.toInt? allows '_' characters.
 -/
-def toInt?' (str : String) : Option Int :=
+public def toInt?' (str : String) : Option Int :=
   if str.contains '_' then .none else String.toInt? str
 
 /--
 Helper function that wraps String.toNat? but returns .none if the string contains '_'.
 This prevents the undocumented behavior where String.toNat? allows '_' characters.
 -/
-def toNat?' (str : String) : Option Nat :=
+public def toNat?' (str : String) : Option Nat :=
   if str.contains '_' then .none else String.toNat? str
